with_fp working... but requires annotations

examples/csl/SL.Actions.fst
@@ -22,19 +22,19 @@ let read_wp (#a:Type) (r:ref a) : st_wp a =
 
 unfold
 let frame_read_wp (#a:Type) (r:ref a) : st_wp a =
-   fun post m0 -> frame_wp (read_wp r) (frame_post post) m0
+   fun post m0 -> frame_wp (with_fp [tosref r] <| read_wp r) (frame_post post) m0
 
 assume
 val ( ! ) (#a:Type) (r:ref a)
-  :STATE a (with_fp [tosref r] <| frame_read_wp r)
+  :STATE a (frame_read_wp r)
 
 let write_wp (#a:Type) (r:ref a) (v:a) : st_wp unit =
   (fun post m0 -> exists (x:a). m0 == (r |> x) /\ post () (r |> v))
 
 unfold
 let frame_write_wp (#a:Type) (r:ref a) (v:a) : st_wp unit =
-   fun post m0 -> frame_wp (write_wp r v) (frame_post post) m0
+   fun post m0 -> frame_wp (with_fp [tosref r] <| write_wp r v) (frame_post post) m0
 
 assume
 val ( := ) (#a:Type) (r:ref a) (v:a)
-  :STATE unit (with_fp [tosref r] <| frame_write_wp r v)
+  :STATE unit (frame_write_wp r v)
