examples/csl/SL.ExamplesAuto.fst
@@ -3,11 +3,11 @@ module SL.ExamplesAuto
 open SL.Base
 open SL.AutoTactic
 
-effect ST (a:Type) (wp:st_wp a) = STATE a (fun post m -> frame_wp wp (frame_post post) m)
+effect ST (a:Type) (wp:st_wp a) (fp:refs) = STATE a (fun post m -> frame_wp (with_fp fp wp) (frame_post post) m)
 
 let swap_wp (r1 r2:ref int) = fun p m -> exists x y. m == (r1 |> x <*> r2 |> y) /\ p () (r1 |> y <*> r2 |> x)
 
-let swap (r1 r2:ref int) : ST unit (swap_wp r1 r2) by (sl_auto ())
+let swap (r1 r2:ref int) : ST unit (swap_wp r1 r2) [tosref r1; tosref r2] by (sl_auto ())
   = let x = !r1 in
     let y = !r2 in
     r1 := y;
@@ -16,34 +16,34 @@ let swap (r1 r2:ref int) : ST unit (swap_wp r1 r2) by (sl_auto ())
 let rotate_wp (r1 r2 r3:ref int)
   = fun p m -> exists x y z. m == (r1 |> x <*> r2 |> y <*> r3 |> z) /\ p () (r1 |> z <*> r2 |> x <*> r3 |> y)
 
-let rotate (r1 r2 r3:ref int) : ST unit (rotate_wp r1 r2 r3) by (sl_auto ())
+let rotate (r1 r2 r3:ref int) : ST unit (rotate_wp r1 r2 r3) [tosref r1; tosref r2; tosref r3] by (sl_auto ())
   = swap r2 r3;
     swap r1 r2
 
-let test (r1 r2:ref int) : ST int (fun p m -> exists x y. m == (r1 |> x <*> r2 |> y) /\ p x m) by (sl_auto ())
+let test (r1 r2:ref int) : ST int (fun p m -> exists x y. m == (r1 |> x <*> r2 |> y) /\ p x m) [tosref r1; tosref r2] by (sl_auto ())
   = !r1
 
 (*
  * two commands
  *)
-let write_read (r1 r2:ref int) : ST int (fun p m -> exists x y. m == (r1 |> x <*> r2 |> y) /\ p y (r1 |> 2 <*> r2 |> y)) by (sl_auto ())
+let write_read (r1 r2:ref int) : ST int (fun p m -> exists x y. m == (r1 |> x <*> r2 |> y) /\ p y (r1 |> 2 <*> r2 |> y)) [tosref r1; tosref r2] by (sl_auto ())
   = r1 := 2;
     !r2
 
-let read_write (r1 r2:ref int) : ST unit (fun p m -> exists x y. m == (r1 |> x <*> r2 |> y) /\ p () (r1 |> x <*> r2 |> x)) by (sl_auto ())
+let read_write (r1 r2:ref int) : ST unit (fun p m -> exists x y. m == (r1 |> x <*> r2 |> y) /\ p () (r1 |> x <*> r2 |> x)) [tosref r1; tosref r2] by (sl_auto ())
   = let x = !r1 in
     r2 := x
 
 let cond_test (r:ref int) (b:bool) : ST unit (fun p m -> exists x. m == r |> x /\ ((b   ==> p () (r |> 1)) /\
-                                                                      (~ b ==> p () (r |> 2))))
-  by (prelude' (); sl 0)
+                                                                      (~ b ==> p () (r |> 2)))) [tosref r]
+  by (sl_auto ())
 
   = if b then r := 1 else r := 2
 
 let rotate_left_or_right (r1 r2 r3:ref int) (b:bool)
   : ST unit (fun p m -> exists x y z. m == (r1 |> x <*> r2 |> y <*> r3 |> z) /\
                               ((b   ==> p () (r1 |> z <*> r2 |> x <*> r3 |> y)) /\
- 			      (~ b ==> p () (r1 |> y <*> r2 |> z <*> r3 |> x))))
+ 			      (~ b ==> p () (r1 |> y <*> r2 |> z <*> r3 |> x)))) [tosref r1; tosref r2; tosref r3]
   by (sl_auto ())
 
   = if b then rotate r1 r2 r3 else rotate r3 r2 r1
